\begin{figure}[ht]
	\centering
	\begin{subfigure}[b]{0.45\textwidth}
		\centering
		\begin{tikzpicture}
			\node[box] (con1) at (-.5,0) {$A$};
			\node[box] (per1) at (-.5,-1) {$B$};
			\node[box] (con2) at (.5,0) {$C$};
			\node[box] (per2) at (.5,-1) {$D$};
			\draw[->] (per1) -- (con1);
			\draw[->] (per2) -- (con2);
		\end{tikzpicture}
		\figsentence{$A$ because $B$ and $C$ because $D$.}
	\end{subfigure}
	\begin{subfigure}[b]{0.45\textwidth}
		\centering
		\begin{tikzpicture}
			\node[box] (con) at (0,0) {$A$};
			\node[box] (per1) at (-.5,-1) {$B$};
			\node[box] (per2) at (.5,-1) {$C$};
			\node[box] (per3) at (.5,-2) {$D$};
			\draw[->] (per1) -- ++(0,.4) -| (con);
			\draw[->] (per2) -- ++(0,.4) -| (con);
			\draw[->] (per3) -> (per2);
		\end{tikzpicture}
		\figsentence{$A$ because $B$ and $C$ because $D$.}
	\end{subfigure}
	\caption{Ambiguous cases with recursion and conjunction}
\end{figure}

\begin{figure}
	\centering
	\begin{subfigure}[b]{0.45\textwidth}
		\centering
		\begin{tikzpicture}
			\node[box] (con) at (0,0) {$A$};
			\node[box] (per1) at (0,-1) {$B$};
			\node[box] (per2) at (0,-2) {$C$};
			\draw[->] (per1) -> (con);
			\draw[-x] (per2) -> (per1);
		\end{tikzpicture}
		\figsentence{$A$ because $B$ but $C$.}
		\caption{}
	\end{subfigure}
	\begin{subfigure}[b]{0.45\textwidth}
		\centering
		\begin{tikzpicture}
			\node[box] (con) at (0,0) {$A$};
			\node[box] (per1) at (-.5,-1) {$B$};
			\node[box] (per2) at (.5,-1) {$C$};
			\draw[->] (per1.north) -- ++(0,.2) -| ([xshift=-0.1cm]con.south);
			\draw[-x] (per2.north) -- ++(0,.2) -| ([xshift=0.1cm]con.south);
		\end{tikzpicture}
		\figsentence{$A$ because $B$ but $C$.}
		\caption{}
	\end{subfigure}
	\caption{Ambiguous cases with recursion and rules}
\end{figure}